Environments.v
@@ -1,0 +1,122 @@
+Create HintDb types discriminated.
+Hint Extern 1 => unfold not in *: types.
+
+Record fenv {Key Value: Type} :=
+  { fn :> Key -> Value -> Prop;
+    uniq: forall k v v', fn k v -> fn k v' -> v = v' }.
+
+Arguments fenv: clear implicits.
+Hint Resolve @uniq : types.
+
+Definition fenv_nil {Key Value: Type} : fenv Key Value :=
+  {| fn k v := False;
+     uniq := ltac:(cbv in *; tauto) |}.
+
+Definition fenv_add {Key Value: Type} (env: fenv Key Value) (k: Key) (v: Value) : fenv Key Value.
+  refine {| fn := (fun k' v' => (k = k' /\ v = v') \/ (k <> k' /\ env.(fn) k' v')) |};
+    abstract (destruct env; intuition (subst; eauto with types)).
+Defined.
+
+Definition fenv_le {Key Value: Type} (cmp : Value -> Value -> Prop) (Gamma Gamma': fenv Key Value) :=
+  forall k v, Gamma k v -> exists v', Gamma' k v' /\ cmp v v'.
+
+Class Env {K V: Type}: Type :=
+  { env_t: Type;
+    env_nil: env_t;
+    getenv: env_t -> K -> option V;
+    putenv: env_t -> K -> V -> env_t;
+    getenv_nil: forall k, getenv env_nil k = None;
+    get_put_eq: forall ev k v, getenv (putenv ev k v) k = Some v;
+    get_put_neq: forall ev k k' v, k <> k' -> getenv (putenv ev k v) k' = getenv ev k';
+    get_put_Some: forall ev k k' v v',
+        getenv (putenv ev k v) k' = Some v' ->
+        k = k' /\ v = v' \/ k <> k' /\ getenv ev k' = Some v';
+    get_put_None: forall ev k k' v,
+        getenv (putenv ev k v) k' = None ->
+        k <> k' /\ getenv ev k' = None
+  }.
+Arguments Env : clear implicits.
+Arguments env_t {_ _}.
+
+Section EnvEquiv.
+  Context {K V V': Type} {Env: Env K V}.
+  Context (f: V -> V').
+
+  Definition env_equiv (Gamma: fenv K V') (gamma: env_t Env) :=
+    (forall var v, getenv gamma var = Some v -> Gamma var (f v)) /\
+    (forall var, getenv gamma var = None -> forall tau, not (Gamma var tau)).
+
+  Lemma env_equiv_putenv:
+    forall (Gamma: fenv K V') (gamma: env_t _)
+      (k: K) (v': V') (v: V),
+      f v = v' ->
+      env_equiv Gamma gamma ->
+      env_equiv (fenv_add Gamma k v') (putenv gamma k v).
+  Proof.
+    unfold env_equiv; cbn. intros * ? (H & H') **.
+    split; intros; [
+      pose proof (get_put_Some _ _ _ _ _ ltac:(eassumption)) |
+      pose proof (get_put_None _ _ _ _ ltac:(eassumption))
+    ]; firstorder (subst; eauto).
+  Qed.
+
+  Lemma env_equiv_getenv_Some:
+    forall (Gamma: fenv K V') (k: K) (gamma: env_t _),
+      env_equiv Gamma gamma ->
+      forall v: V,
+        getenv gamma k = Some v ->
+        Gamma k (f v).
+  Proof. firstorder. Qed.
+
+  Lemma env_equiv_getenv_None:
+    forall (Gamma: fenv K V') (k: K) (gamma: env_t _),
+      env_equiv Gamma gamma ->
+      getenv gamma k = None ->
+      forall v', Gamma k v' -> False.
+  Proof. firstorder. Qed.
+
+  Definition tenv_of_env (ev: env_t Env): fenv K V'.
+    refine {| fn k v' := exists v, getenv ev k = Some v /\ v' = f v |}.
+    abstract (intros * (? & Heq & Hfeq) (? & Heq' & Hfeq'); subst;
+              rewrite Heq in Heq'; inversion Heq'; eauto).
+  Defined.
+
+  Lemma tenv_of_env_equiv :
+    forall (ev: env_t Env),
+      env_equiv (tenv_of_env ev) ev.
+  Proof.
+    intros; unfold env_equiv, tenv_of_env, not; cbn; split.
+    - firstorder.
+    - intros * Heq * Hex; rewrite Heq in Hex;
+        firstorder discriminate.
+  Qed.
+
+  Lemma tenv_of_env_nil :
+    env_equiv fenv_nil env_nil.
+    unfold env_equiv, fenv_nil; cbn; split; intros.
+    - rewrite getenv_nil in H; discriminate.
+    - tauto.
+  Qed.
+End EnvEquiv.
+
+Lemma fenv_le_refl {Key Value: Type}:
+  forall (cmp: _ -> _ -> Prop) (Gamma : fenv Key Value),
+    (forall x, cmp x x) ->
+    fenv_le cmp Gamma Gamma.
+Proof.
+  firstorder.
+Qed.
+
+Hint Resolve fenv_le_refl : types.
+
+Lemma fenv_add_increasing {Key Value: Type}:
+  forall (cmp: _ -> _ -> Prop) (Gamma1 : fenv Key Value) (var : Key) (tau tau' : Value) (Gamma2 : fenv Key Value),
+    cmp tau tau' ->
+    fenv_le cmp Gamma1 Gamma2 ->
+    fenv_le cmp (fenv_add Gamma1 var tau) (fenv_add Gamma2 var tau').
+Proof.
+  unfold fenv_le, fenv_add; simpl; firstorder (subst; eauto with types).
+Qed.
+
+Hint Resolve fenv_add_increasing : types.
+
