Syntax.v
@@ -21,3 +21,36 @@ Inductive scheduler {TVar TFn} :=
 | Try (r: rule TVar TFn) (s1 s2: scheduler).
 
 Arguments scheduler : clear implicits.
+
+Require Import List.
+
+(* Better induction principle *)
+Definition rule_ind' {TVar TFn : Type} (P : rule TVar TFn -> Prop)
+           (f : forall (var : TVar) (expr : rule TVar TFn),
+               P expr -> forall body : rule TVar TFn, P body -> P (Bind var expr body))
+           (f0 : forall var : TVar, P (Var var)) (f1 : P Skip) (f2 : forall cst : bits, P (Const cst))
+           (f3 : forall cond : rule TVar TFn,
+               P cond ->
+               forall tbranch : rule TVar TFn,
+                 P tbranch -> forall fbranch : rule TVar TFn, P fbranch -> P (If cond tbranch fbranch))
+           (f4 : P Fail) (f5 : forall (level : Level) (idx : nat), P (Read level idx))
+           (f6 : forall (level : Level) (idx : nat) (value : rule TVar TFn), P value -> P (Write level idx value))
+           (f7: forall (fn : TFn) (args : list (rule TVar TFn)),
+               List.Forall P args ->
+               P (Call fn args)) : forall r, P r.
+  refine (fix F (r : rule TVar TFn) : P r :=
+            match r as r0 return (P r0) with
+            | Bind var expr body => f var expr (F expr) body (F body)
+            | Var var => f0 var
+            | Skip => f1
+            | Const cst => f2 cst
+            | If cond tbranch fbranch => f3 cond (F cond) tbranch (F tbranch) fbranch (F fbranch)
+            | Fail => f4
+            | Read level idx => f5 level idx
+            | Write level idx value => f6 level idx value (F value)
+            | Call fn args => f7 fn args _
+            end).
+  revert args.
+  fix fargs 1.
+  destruct args; cbn; econstructor; eauto.
+Defined.
